WIP

nondeterministic_dataflow/Operator_Examples.thy
@@ -51,15 +51,16 @@ inductive_cases small_production_spec_ConsE[elim!]: "small_production_spec P sta
 
 
 coinductive production_spec for P where
-  "P state [] [] state \<Longrightarrow> production_spec P state LNil"
+  "production_spec P state LNil"
 | "production_spec P state' lxs \<Longrightarrow> P state ins out state' \<Longrightarrow>
    (\<forall> x \<in> set ins. is_VInp x) \<Longrightarrow> (\<forall> x \<in> set out. \<not> is_VInp x) \<Longrightarrow>
    ins @ out \<noteq> [] \<Longrightarrow> production_spec P state (ins @- out @- lxs)"
-
+(* 
 inductive_cases production_spec_LNilE[elim!]: "production_spec P state LNil"
 inductive_cases production_spec_shiftE[elim!]: "production_spec P state (ins @- out @- lxs)"
 inductive_cases production_spec_ConsVInpE[elim!]: "production_spec P state (LCons (VInp p x) lxs)"
 inductive_cases production_spec_ConsVOutE[elim!]: "production_spec P state (LCons (VOut p x) lxs)"
+ *)
 
 lemma step_empty_writes:
   "step io (writes op p []) op' \<Longrightarrow> step io op op'"
@@ -496,8 +497,15 @@ lemma filter_op_correctness_alt:
    wtraced (filter_op P buf) lxs = production_spec (\<lambda>buf inps outs buf'. bulk_benq (map (case_VIO VOut VOut) (filter (case_VIO (\<lambda>_. P) \<top>) inps)) (map (VOut 1) buf) = bulk_benq (map (VOut 1) buf') outs) buf lxs"
   using wtraced_production_spec_completeness wtraced_production_spec_soundness by blast
 
+definition state_invar where
+  "state_invar R =  (\<forall> op op' io state. step io op' op \<longrightarrow> R op state \<longrightarrow> (\<exists> state'. R op' state'))"
+
 definition operator_spec where                                   
-  "operator_spec op state spec = (\<forall> lxs. wtraced op lxs \<longleftrightarrow> production_spec spec state lxs)"
+  "operator_spec op R Q \<longleftrightarrow> (\<forall> lxs state. R op state \<longrightarrow> wtraced op lxs \<longrightarrow> small_production_spec Q state lxs)"
+
+
+definition hoare where                                   
+  "hoare P C Q \<longleftrightarrow> (\<forall> io state state'. P state \<longrightarrow> wstep io (C state) (C state') \<longrightarrow> Q state' io)"
 
 lemma filter_op_correctness:
   "\<forall> x \<in> set buf. P x \<Longrightarrow>
@@ -540,39 +548,42 @@ lemma
       oops
 
 lemma
-  "step io op1 op1' \<Longrightarrow>
-   operator_spec op1 s1 P1 \<Longrightarrow>
-   \<exists> s1'. operator_spec op1' s1' P1"
+  "step io op op' \<Longrightarrow>
+   io \<noteq> Tau \<Longrightarrow>
+   state_invar R \<Longrightarrow>
+   operator_spec op R Q \<Longrightarrow>
+   operator_spec op' R Q"
   apply (subst operator_spec_def)
   subgoal
-    apply (rule exI)
     apply safe
-    oops
-(*   apply (intro allI iffI)
-  subgoal for lxs
-    apply (coinduction arbitrary: s1 s1' op1 lxs rule: production_spec.coinduct)
-    subgoal for s1 s1' op1 lxs                                
-      apply (cases io)
-      subgoal for p x
-        apply hypsubst_thin
-        apply (drule spec[of _ "LCons (VInp p x) lxs"])
-        apply (auto del: disjCI)
-        subgoal for state' lxs' ins out op'
-          apply (cases lxs)
-          subgoal
-            apply simp
-            apply hypsubst_thin
-            apply (cases out; cases lxs'; cases ins; simp; hypsubst_thin)
-            subgoal for xs
-              apply (rule disjI2)
-              apply (rule exI[of _ state'])
-              apply (rule exI[of _ LNil])
-              apply (rule exI[of _ Nil])
-              apply (rule exI[of _ Nil])
-              apply simp
-              apply (cases xs; simp)
-              apply auto
-  oops *)
+    subgoal for lxs state
+      apply (subst (asm) operator_spec_def)
+      apply (drule spec[of _ "LCons (vio_of_io io) lxs"])
+      unfolding state_invar_def
+      apply (drule spec[of _ op'])
+      apply (drule spec[of _ op])
+      apply (drule spec[of _ io])
+      apply (drule spec[of _ state])
+      back
+      apply simp
+      apply auto
+      subgoal for state'
+        apply (drule spec[of _ state'])
+        apply simp
+        apply (drule mp)
+         apply (metis step_wstep vio_of_io_inverse wtraced.Step)
+        apply (erule small_production_spec.cases)
+        apply auto
+
+      done
+    done
+  done
+
+      apply (erule production_spec.cases)  
+       apply force
+      apply (rule exI[of)
+
+      oops
 
 lemma comp_op_spec_empty:
   "P1 s1 [] [] s1 \<Longrightarrow>
@@ -683,7 +694,7 @@ lemma
   subgoal for lxs
         apply (drule spec[of _ "LCons (VInp p x) lxs"])
     apply auto
-    sledgehammer
+    oops
 
 
 end
