nondeterministic_dataflow/Wtraced_Composition.thy
@@ -395,7 +395,7 @@ lemma wstep_comp_op_wfinished_preserve:
     done
   done
 
-lemma
+lemma wtraced_comp_op:
   "wtraced (comp_op wire buf op1 op2) ios = 
    (\<exists> ios1 ios2. wtraced op1 ios1 \<and> wtraced op2 ios2 \<and> causal wire buf ios ios1 ios2)"
   apply (rule iffI)
@@ -441,6 +441,418 @@ lemma
       done
     done
   done
+
+
+lemma wtraced_map_op: 
+ "inj_on f (inputs op) \<Longrightarrow>
+  inj_on g (outputs op) \<Longrightarrow>
+  wtraced (map_op f g op) lxs = (\<exists>lys. wtraced op lys \<and> lxs = lmap (map_VIO f g id) lys)"
+  sorry
+
+
+corec filter_op where
+  "filter_op P buf = choice2 
+   (Read (1 :: 1) (\<lambda> x. filter_op P (if P x then buf @ [x] else buf)))
+   (if buf = [] then filter_op P buf else Write (filter_op P (tl buf)) (1 :: 1) (hd buf))"
+
+coinductive production_spec for P where
+  "production_spec P state LNil"
+| "production_spec P state' lxs \<Longrightarrow> P state ins out state' \<Longrightarrow>
+   (\<forall> x \<in> set ins. is_VInp x) \<Longrightarrow> (\<forall> x \<in> set out. \<not> is_VInp x) \<Longrightarrow>
+   ins @ out \<noteq> [] \<Longrightarrow> production_spec P state (ins @- out @- lxs)"
+
+lemma step_Inp_True_filter_op:
+  "step io op op' \<Longrightarrow>
+   io = Inp p x \<Longrightarrow>
+   op = filter_op P buf \<Longrightarrow>
+   P x \<Longrightarrow>
+   p = 1 \<and> op' = filter_op P (buf @ [x])"
+  apply (induct io op op' arbitrary: buf pred: step)
+     apply (subst (asm) filter_op.code, simp)    
+    apply (subst (asm) filter_op.code, simp)
+   apply (subst (asm) filter_op.code, simp)
+  subgoal for op ops io op' buf
+    apply hypsubst_thin
+    apply (subst (asm) (3) filter_op.code)
+    apply (auto split: op.splits list.splits if_splits ; hypsubst_thin)
+    done
+  done
+
+lemma step_Inp_False_filter_op:
+  "step io op op' \<Longrightarrow>
+   io = Inp p x \<Longrightarrow>
+   op = filter_op P buf \<Longrightarrow>
+   \<not> P x \<Longrightarrow>
+   p = 1 \<and> op' = filter_op P buf"
+  apply (induct io op op' arbitrary: buf pred: step)
+     apply (subst (asm) filter_op.code, simp)    
+    apply (subst (asm) filter_op.code, simp)
+   apply (subst (asm) filter_op.code, simp)
+  subgoal for op ops io op' buf
+    apply hypsubst_thin
+    apply (subst (asm) (3) filter_op.code)
+    apply (auto split: op.splits list.splits if_splits ; hypsubst_thin)
+    done
+  done
+
+lemma step_Tau_filter_op:
+  "step io op op' \<Longrightarrow>
+   io = Tau \<Longrightarrow>
+   op = filter_op P buf \<Longrightarrow>
+   False"
+  apply (induct io op op' arbitrary: buf pred: step)
+     apply (subst (asm) filter_op.code, simp)    
+    apply (subst (asm) filter_op.code, simp)
+   apply (subst (asm) filter_op.code, simp)
+  subgoal for op ops io op' buf
+    apply hypsubst_thin
+    apply (subst (asm) (2) filter_op.code)
+    apply (fastforce split: if_splits op.splits list.splits; hypsubst_thin)
+    done
+  done
+
+lemma wstep_Inp_True_filter_op:
+  "wstep io op op' \<Longrightarrow>
+   io = Inp p x \<Longrightarrow>
+   op = filter_op P buf \<Longrightarrow>
+   P x \<Longrightarrow>
+   p = 1 \<and> op' = filter_op P (buf @ [x])"
+  unfolding wstep_def
+  apply (metis (mono_tags, lifting) converse_rtranclpE estep.simps(2) relcompp_apply step_Inp_True_filter_op step_Tau_filter_op)
+  done
+
+lemma wstep_Inp_False_filter_op:
+  "wstep io op op' \<Longrightarrow>
+   io = Inp p x \<Longrightarrow>
+   op = filter_op P buf \<Longrightarrow>
+   \<not> P x \<Longrightarrow>
+   p = 1 \<and> op' = filter_op P buf"
+  unfolding wstep_def
+  apply (metis converse_rtranclpE estep.simps(2) pick_middlep step_Inp_False_filter_op step_Tau_filter_op)
+  done
+
+lemma step_Out_filter_op:
+  "step io op op' \<Longrightarrow>
+   io = Out p x \<Longrightarrow>
+   op = filter_op P buf \<Longrightarrow>
+   p = 1 \<and> op' = filter_op P (tl buf) \<and> buf \<noteq> [] \<and> bhd buf = x"
+  apply (induct io op op' arbitrary: buf pred: step)
+     apply (subst (asm) filter_op.code, simp)    
+    apply (subst (asm) filter_op.code, simp)
+   apply (subst (asm) filter_op.code, simp)
+  subgoal for op ops io op' buf
+    apply hypsubst_thin
+    apply (subst (asm) (3) filter_op.code)
+    apply simp
+    apply hypsubst_thin
+    apply (elim disjE)
+     apply hypsubst_thin
+     apply force
+    apply hypsubst_thin
+    apply (cases buf; simp)
+     apply blast
+    apply (auto split: if_splits)
+    done
+  done
+
+lemma step_Inp_True_filter_op_intro:
+  "buf' = bulk_benq [x] buf \<Longrightarrow>
+   P x \<Longrightarrow>
+   step (Inp 1 x) (filter_op P buf) (filter_op P buf')"
+  apply (subst filter_op.code)
+  apply (simp split: if_splits)
+  apply (intro conjI impI)
+   apply (rule SC)
+    apply (rule cinsertI1)
+   apply (smt (verit, del_insts) SR self_append_conv2)
+  apply (rule SC)
+   apply (rule cinsertI1)
+  apply (smt (verit, del_insts) SR self_append_conv2)
+  done  
+
+lemma step_Inp_False_filter_op_intro:
+  "\<not> P x \<Longrightarrow>
+   step (Inp 1 x) (filter_op P buf) (filter_op P buf)"
+  apply (subst filter_op.code)
+  apply (simp split: if_splits)
+  apply (intro conjI impI)
+   apply (rule SC)
+    apply (rule cinsertI1)
+   apply (smt (verit, del_insts) SR self_append_conv2)
+  apply (rule SC)
+   apply (rule cinsertI1)
+  apply (smt (verit, del_insts) SR self_append_conv2)
+  done  
+
+lemma step_Out_filter_op_intro:
+  "buf' = tl buf \<Longrightarrow>
+   buf \<noteq> [] \<Longrightarrow>
+   hd buf = x \<Longrightarrow>
+   step (Out 1 x) (filter_op P buf) (filter_op P buf')"
+  apply (subst filter_op.code)
+  apply (simp split: if_splits)
+  apply (rule SC)
+   apply (rule cinsertI2)
+   apply (rule cinsertI1)
+  apply blast
+  done
+
+lemma wstep_Out_filter_op:
+  "wstep io op op' \<Longrightarrow>
+   io = Out p x \<Longrightarrow>
+   op = filter_op P buf \<Longrightarrow>
+   p = 1 \<and> op' = filter_op P (tl buf)\<and> buf \<noteq> [] \<and> bhd buf = x"
+  unfolding wstep_def by (metis (no_types, lifting) converse_rtranclpE estep.simps(3) pick_middlep step_Out_filter_op step_Tau_filter_op)
+
+lemma wtraced_production_spec_soundness:
+  "\<forall> x \<in> set buf. P x \<Longrightarrow>
+   wtraced (filter_op P buf) lxs \<Longrightarrow>
+   production_spec (\<lambda> buf inps outs buf'. (length outs = 1 \<and> inps = [] \<or> length inps = 1 \<and> outs = []) \<and> map (VOut 1) buf @ map (case_VIO VOut VOut) (filter (case_VIO (\<lambda> _ x. P x) \<top>) inps) = outs @ map (VOut 1) buf') buf lxs"
+  apply (coinduction arbitrary: buf lxs rule: production_spec.coinduct)
+  subgoal for buf lxs
+    apply (erule wtraced.cases)
+    subgoal for op
+      by (cases buf; simp)
+    subgoal for vio op op' lxs'
+      apply hypsubst_thin
+      apply (cases vio; simp; hypsubst_thin?)
+      subgoal for p x
+        apply (cases "P x")
+        subgoal
+          apply (rule exI[of _ "buf @ [x]"])
+          apply (rule exI[of _ "lxs'"])
+          apply (rule exI[of _ "[VInp p x]"])
+          apply (rule exI[of _ "[]"])
+          apply simp
+          apply (intro disjI1 conjI)
+          using wstep_Inp_True_filter_op apply force
+          done
+        subgoal
+          apply (rule exI[of _ "buf"])
+          apply (rule exI[of _ "lxs'"])
+          apply (rule exI[of _ "[VInp p x]"])
+          apply (rule exI[of _ "[]"])
+          apply simp
+          apply (intro disjI1 conjI)
+          using wstep_Inp_False_filter_op apply force
+          done
+        done
+      subgoal for p x
+        apply (drule wstep_Out_filter_op)
+          apply (rule refl)+
+        apply safe
+        apply (rule exI[of _ "btl buf"])
+        apply (rule exI[of _ "lxs'"])
+        apply (rule exI[of _ "[]"])
+        apply (rule exI[of _ "[VOut p x]"])
+        apply simp
+        apply (intro disjI1 conjI)
+         apply (metis list.set_sel(2))
+        apply (metis (full_types) list.exhaust_sel list.simps(9) num1_eq1)
+        done
+      done
+    done
+  done  
+
+
+lemma wtraced_production_spec_completeness:
+  "\<forall> x \<in> set buf. P x \<Longrightarrow>
+   production_spec (\<lambda> buf inps outs buf'. (length outs = 1 \<and> inps = [] \<or> length inps = 1 \<and> outs = []) \<and> map (VOut 1) buf @ map (case_VIO VOut VOut) (filter (case_VIO (\<lambda> _ x. P x) \<top>) inps) = outs @ map (VOut 1) buf') buf lxs \<Longrightarrow>
+   wtraced (filter_op P buf) lxs"
+  apply (coinduction arbitrary: buf lxs rule: wtraced.coinduct)
+  subgoal for buf lxs
+    apply (erule production_spec.cases)
+    subgoal
+      by blast
+    subgoal for buf' lxs buf ins out
+      apply hypsubst_thin
+      apply (cases out; cases ins;  simp split: if_splits VIO.splits)
+      subgoal for i p x
+        apply (rule exI[of _ "filter_op P (buf @ [x])"])
+        apply (intro conjI)
+        subgoal
+          apply hypsubst_thin
+          using step_Inp_True_filter_op_intro apply (metis (full_types) num1_eq1 step_wstep)
+          done
+        apply (rule disjI1)
+        apply (rule exI[of _ "buf @ [x]"])
+        apply simp
+         apply (smt (verit, best) Cons_eq_map_conv VIO.inject(2) list.inj_map_strong map_eq_append_conv map_is_Nil_conv)
+        done
+      subgoal for ins' p x
+        apply hypsubst_thin
+        apply (rule exI[of _ "filter_op P buf"])
+        apply (intro conjI)
+        subgoal
+          using step_Inp_False_filter_op_intro apply (metis (full_types) num1_eq1 step_wstep)
+          done
+        apply (rule disjI1)
+        apply (rule exI[of _ "buf"])
+        apply simp
+         apply (smt (verit, best) Cons_eq_map_conv VIO.inject(2) list.inj_map_strong map_eq_append_conv map_is_Nil_conv)
+        done
+      subgoal for oo 
+        apply hypsubst_thin
+        apply (cases oo; simp; hypsubst_thin)
+        subgoal for p x
+          apply (rule exI[of _ "filter_op P (tl buf)"])
+          apply (intro conjI)
+          subgoal
+            using step_Out_filter_op_intro apply force
+            done
+          apply (rule disjI1)
+          apply (rule exI[of _ "tl buf"])
+          apply simp
+          apply (intro conjI)
+           apply force
+           apply (smt (verit, ccfv_SIG) VIO.inject(2) list.inj_map_strong list.sel(3) map_tl)
+          done
+        done
+      done
+    done
+  done
+
+lemma filter_op_correctness:
+  "\<forall>x\<in>set buf. P x \<Longrightarrow>
+   wtraced (filter_op P buf) lxs = production_spec (\<lambda>buf inps outs buf'. (length outs = 1 \<and> inps = [] \<or> length inps = 1 \<and> outs = []) \<and> bulk_benq (map (case_VIO VOut VOut) (filter (case_VIO (\<lambda>_. P) \<top>) inps)) (map (VOut 1) buf) = bulk_benq (map (VOut 1) buf') outs) buf lxs"
+  using wtraced_production_spec_completeness wtraced_production_spec_soundness by blast
+
+simproc_setup num1_eq (\<open>x :: 1\<close>) =
+  \<open>K (K (fn ct =>
+    if Thm.term_of ct aconv @{term \<open>1 :: 1\<close>} then NONE
+    else SOME (mk_meta_eq @{thm num1_eq1})))\<close>
+
+thm production_spec.coinduct[no_vars]
+
+lemma production_spec_coinduct:
+  "X x1 x2 \<Longrightarrow>
+(\<And>x1 x2.
+    X x1 x2 \<Longrightarrow>
+    (\<exists>state. x1 = state \<and> x2 = LNil) \<or>
+    (\<exists>state' lxs state ins out.
+        x1 = state \<and>
+        x2 = ins @- out @- lxs \<and>
+        (X state' lxs) \<and>
+        P state ins out state' \<and> Ball (set ins) is_VInp \<and> (\<forall>x\<in>set out. \<not> is_VInp x) \<and> bulk_benq out ins \<noteq> [])) \<Longrightarrow>
+  production_spec P x1 x2"
+  apply (erule production_spec.coinduct)
+  apply blast
+  done
+
+lemma
+  "\<forall>x\<in>set buf1. P x \<Longrightarrow>
+   \<forall>x\<in>set buf2. P x \<Longrightarrow>
+   \<forall>x\<in>set buf3. P x \<and> Q x \<Longrightarrow>
+   wtraced (map_op projl projr (comp_op Some (\<lambda>_. buf2) (filter_op P buf1) (filter_op Q buf3))) lxs =
+   production_spec (\<lambda>buf inps outs buf'. (length outs = 1 \<and> inps = [] \<or> length inps = 1 \<and> outs = []) \<and> bulk_benq (map (case_VIO VOut VOut) (filter (case_VIO (\<lambda>p x. P x \<and> Q x) \<top>) inps)) (map (VOut 1) buf) = bulk_benq (map (VOut 1) buf') outs) (buf3 @ buf2 @ buf1) lxs"
+  unfolding scomp_op_def
+  apply (subst wtraced_map_op)
+  subgoal
+    apply (rule inj_onI)
+    apply auto
+    done
+  subgoal
+    apply (rule inj_onI)
+    apply auto
+    done
+  apply (subst wtraced_comp_op)
+  apply (rule iffI)
+  subgoal
+    apply (elim conjE exE)
+    apply hypsubst_thin
+    subgoal for lys ios1 ios2
+      apply (coinduction arbitrary: buf1 buf2 buf3 ios1 ios2 lys rule: production_spec_coinduct)
+      subgoal for buf1 buf2 buf3 ios1 ios2 lys
+        apply simp
+        apply (erule causal.cases)
+        subgoal
+          by simp
+        subgoal for buf' ios' ios1' ios2' ios buf ios1 ios2
+          apply hypsubst_thin
+          apply simp
+          apply (rule disjI2)
+          subgoal premises prems
+            using prems(8,1-7) apply -
+          apply (induct "\<lambda> _ :: 1. buf2" ios ios1 ios2 buf' ios' ios1' ios2' arbitrary: buf1 buf2 buf3 rule: visible_cause.induct)
+               apply simp_all
+          subgoal for x iosa ios1 ios2 buf2 buf1 buf3
+            apply (cases "P x"; cases "Q x")
+            subgoal
+            apply (rule exI)
+            apply (rule exI[of _ "lmap (map_VIO projl projr id) iosa"])
+            apply (rule exI[of _ "[VInp 1 x]"])
+            apply (rule exI[of _ "[]"])
+              apply simp
+            apply (intro conjI)
+            apply (rule exI[of _ "buf1 @ [x]"])
+            apply (intro exI)
+            apply (intro conjI)
+              apply (rule refl)
+               apply (intro conjI exI)
+                    apply (rule refl)+
+                   apply simp_all
+              apply (subst filter_op_correctness)
+               apply simp
+              apply (subst (asm) filter_op_correctness)
+               apply simp
+              apply (erule production_spec.cases)
+               apply auto
+               apply (metis (no_types, lifting) VIO.discI(1) list.set_intros(1) llist.inject lshift.elims)
+              subgoal for state' lxs ins
+                apply (cases ins; simp; hypsubst_thin)
+                apply (smt (z3) VIO.inject(2) length_0_conv length_map list.inj_map_strong map_eq_Cons_D map_eq_append_conv)
+                done
+              done
+            subgoal
+              sorry
+     subgoal
+       sorry
+     subgoal
+              sorry
+            done
+          subgoal for x iosa ios1 ios2 buf2 buf1 buf3
+            sorry
+          subgoal premises prems for x ios ios1 ios2 buf' ios1' ios2' buf2 buf1 buf3
+            using prems(1,3-) prems(2)[where ?buf2.0="buf2 @ [x]" and ?buf1.0="tl buf1" and ?buf3.0=buf3] apply (auto simp: fun_eq_iff)
+            apply (drule meta_mp)
+             apply (metis list.sel(2) list.set_sel(2))
+            apply (drule meta_mp)
+            apply (metis list.collapse list.set_intros(1) wstep_Out_filter_op)
+            apply (drule meta_mp)
+             apply (metis wstep_Out_filter_op)
+            apply (elim exE conjE)
+            subgoal for op' state' lxs ins out buf1 buf2 buf3 ios1 ios2 lys
+              apply hypsubst
+              apply (rule exI[of _ state'])
+              apply (rule exI[of _ "lmap (map_VIO projl projr id) lys"])
+              apply (rule exI[of _ ins])
+              apply (rule exI[of _ out])
+              apply simp
+              apply (intro conjI)
+              subgoal
+              apply (rule exI[of _ buf1])
+              apply (rule exI[of _ buf2])
+              apply (rule exI[of _ buf3])
+                apply auto
+                done
+              apply (smt (verit, ccfv_SIG) append_Cons list.exhaust_sel list.simps(9) wstep_Out_filter_op)
+              done
+            done
+
+
+end
+
+          apply (rule exI)
+          apply (rule exI[of _ "lmap (map_VIO projl projr id) ios"])
+          apply (rule exI[of _ "[]"])
+          apply (rule exI[of _ "[]"])
+
+
+              oops
+end
+end
+                
+
 
 
 end
